Separate untrusted exec-related proofs

src/Spec/ConcurExec.v
@@ -1,9 +1,10 @@
 Require Export Trace.
 Require Export ConcurProc.
-Require Export FinMap.
+Require Export ExecSemantics.
+Require Export Helpers.FinMap.
+
 Require Import ProofAutomation.
 Require Import Helpers.ListStuff.
-Require Import Helpers.FinMap.
 Require Import Helpers.Instances.
 
 Require Import Relations.Relation_Operators.
@@ -11,116 +12,20 @@ Require Import RelationClasses.
 Require Import Morphisms.
 Require Import FunctionalExtensionality.
 Require Import Omega.
-Require Import List.
 Require Import Bool.
 
-Import ListNotations.
+Section Execution.
 
-Global Set Implicit Arguments.
-Global Generalizable All Variables.
-
-Section Proc.
-
-  Variable Op: Type -> Type.
-  Variable State : Type.
-
-  Definition OpSemantics := forall T, Op T -> nat -> State -> T -> State -> list event -> Prop.
-  Variable op_step : OpSemantics.
-
-  Definition until1 T (c : T -> bool)
-                      (p : option T -> proc Op T)
-                      (v : option T) :=
-    Bind (p v) (fun x => if bool_dec (c x) true then Ret x else Until c p (Some x)).
-
-
-  Inductive atomic_exec : forall T, proc Op T -> nat -> State ->
-                                    T -> State -> list event -> Prop :=
-
-  | AtomicRet : forall T tid (v : T) s,
-    atomic_exec (Ret v) tid s v s nil
-
-  | AtomicBind : forall T1 T2 tid (p1 : proc Op T1) (p2 : T1 -> proc Op T2)
-                        s0 s1 s2 ev1 ev2 (v1 : T1) (v2 : T2),
-    atomic_exec p1 tid s0 v1 s1 ev1 ->
-    atomic_exec (p2 v1) tid s1 v2 s2 ev2 ->
-    atomic_exec (Bind p1 p2) tid s0 v2 s2 (ev1 ++ ev2)
-
-  | AtomicOp : forall T tid (v : T) s s' op evs,
-    op_step op tid s v s' evs ->
-    atomic_exec (Call op) tid s v s' evs
-
-  | AtomicUntil : forall T (p : option T -> proc Op T) (c : T -> bool) v tid s r s' ev',
-    atomic_exec (until1 c p v) tid s r s' ev' ->
-    atomic_exec (Until c p v) tid s r s' ev'
-  .
-
-
-  Inductive exec_tid : forall T (tid : nat),
-    State -> proc Op T ->
-    State -> T + proc Op T -> maybe_proc Op -> list event -> Prop :=
-
-  | ExecTidRet : forall tid T (v : T) s,
-    exec_tid tid s (Ret v)
-                 s (inl v)
-                 NoProc nil
-
-  | ExecTidOp : forall tid T (v : T) s s' op evs,
-    op_step op tid s v s' evs ->
-    exec_tid tid s (Call op)
-                 s' (inl v)
-                 NoProc evs
-
-  | ExecTidAtomic : forall tid T (v : T) ap s s' evs,
-    atomic_exec ap tid s v s' evs ->
-    exec_tid tid s (Atomic ap)
-                 s' (inl v)
-                 NoProc evs
-
-  | ExecTidBind : forall tid T1 (p1 : proc Op T1) T2 (p2 : T1 -> proc Op T2) s s' result spawned evs,
-    exec_tid tid s p1
-                 s' result spawned evs ->
-    exec_tid tid s (Bind p1 p2)
-                 s' (inr
-                     match result with
-                     | inl r => p2 r
-                     | inr p1' => Bind p1' p2
-                     end
-                    ) spawned evs
-
-  | ExecTidUntil : forall tid T (p : option T -> proc Op T) (c : T -> bool) v s,
-    exec_tid tid s (Until c p v)
-                 s (inr (until1 c p v))
-                 NoProc nil
-
-  | ExecTidSpawn : forall tid T (p: proc Op T) s,
-    exec_tid tid s (Spawn p)
-                 s (inl tt)
-                 (Proc p) nil
-  .
-
-
-  Inductive exec : State -> threads_state Op -> trace -> Prop :=
-
-  | ExecOne : forall T tid tid' (ts : threads_state Op) trace p s s' evs result spawned,
-    ts tid = @Proc Op T p ->
-    ts tid' = NoProc ->
-    exec_tid tid s p s' result spawned evs ->
-    exec s' (thread_upd (thread_upd ts tid' spawned) tid
-              match result with
-              | inl _ => NoProc
-              | inr p' => Proc p'
-              end) trace ->
-    exec s ts (prepend tid evs trace)
-
-  | ExecStop : forall (ts : threads_state Op) s,
-    exec s ts TraceEmpty.
+  Variable Op:Type -> Type.
+  Variable State: Type.
+  Variable op_step: OpSemantics Op State.
 
   Inductive exec_till : nat -> State -> threads_state Op -> trace -> Prop :=
 
   | ExecTillOne : forall T tid tid' (ts : threads_state Op) trace p s s' evs result spawned n,
     ts tid = @Proc Op T p ->
     ts tid' = NoProc ->
-    exec_tid tid s p s' result spawned evs ->
+    exec_tid op_step tid s p s' result spawned evs ->
     exec_till n s' (thread_upd (thread_upd ts tid' spawned) tid
               match result with
               | inl _ => NoProc
@@ -132,7 +37,7 @@ Section Proc.
     exec_till 0 s ts TraceEmpty.
 
   Theorem exec_to_counter : forall s ts tr,
-      exec s ts tr ->
+      exec op_step s ts tr ->
       exists n, exec_till n s ts tr.
   Proof.
     induction 1; propositional;
@@ -141,7 +46,7 @@ Section Proc.
 
   Theorem exec_till_to_exec : forall n s ts tr,
       exec_till n s ts tr ->
-      exec s ts tr.
+      exec op_step s ts tr.
   Proof.
     induction 1; propositional;
       eauto using ExecOne, ExecStop.
@@ -155,14 +60,14 @@ Section Proc.
            (tid' : nat) spawned,
          thread_get ts tid = Proc p ->
          thread_get ts tid' = NoProc ->
-         exec_tid tid s p s' result spawned evs ->
-         exec s'
+         exec_tid op_step tid s p s' result spawned evs ->
+         exec op_step s'
            (thread_upd (thread_upd ts tid' spawned) tid
              (match result with
               | inl _ => NoProc
               | inr p' => Proc p'
               end)) tr ->
-         exec s ts (prepend tid evs tr).
+         exec op_step s ts (prepend tid evs tr).
   Proof.
     intros.
     eapply ExecOne; eauto.
@@ -179,11 +84,11 @@ Section Proc.
     exec_any tid s p r s'
   | ExecAnyThisDone :
     forall T (p : proc Op T) (r : T) (s' : State) spawned evs,
-    exec_tid tid s p s' (inl r) spawned evs ->
+    exec_tid op_step tid s p s' (inl r) spawned evs ->
     exec_any tid s p r s'
   | ExecAnyThisMore :
     forall T (p p' : proc Op T) (s' s0 : State) r spawned evs,
-    exec_tid tid s p s0 (inr p') spawned evs ->
+    exec_tid op_step tid s p s0 (inr p') spawned evs ->
     exec_any tid s0 p' r s' ->
     exec_any tid s p r s'
   .
@@ -247,7 +152,7 @@ Section Proc.
   Lemma exec_tid_exec_others :
     forall tid tid' `(p : proc Op T) s s' result spawned evs,
       tid <> tid' ->
-      exec_tid tid' s p s' result spawned evs ->
+      exec_tid op_step tid' s p s' result spawned evs ->
       exec_others tid s s'.
   Proof.
     induction 2; propositional; eauto;
@@ -269,23 +174,12 @@ Section Proc.
     induction 1; propositional; eauto using ExecAnyOther.
   Qed.
 
-End Proc.
+End Execution.
 
-Hint Constructors exec.
 Hint Constructors exec_any.
 Hint Resolve exec_tid_exec_others.
 Hint Resolve exec_others_exec_any.
 Hint Resolve exec_others_trans.
-
-
-Notation "x <- p1 ; p2" := (Bind p1 (fun x => p2))
-  (at level 60, right associativity).
-
-Notation "ts [[ tid ]]" := (thread_get ts tid)
-  (at level 12, left associativity).
-
-Notation "ts [[ tid := p ]]" := (thread_upd ts tid p)
-                                  (at level 12, left associativity).
 
 Section StepImpl.
 
