src/Spec/Abstraction.v
@@ -1,6 +1,4 @@
 Require Import ConcurExec.
-Require Import Relations.Relation_Operators.
-Require Import RelationClasses.
 Require Import Morphisms.
 Require Import ProofAutomation.
 Require Import Helpers.ListStuff.
