src/Spec/ExecSemantics.v
@@ -1,0 +1,116 @@
+Require Import Trace.
+Require Import ConcurProc.
+Require Import Helpers.FinMap.
+
+Global Set Implicit Arguments.
+Global Generalizable All Variables.
+
+Definition bool_dec (x y:bool) : {x=y} + {x<>y}.
+Proof.
+  decide equality.
+Defined.
+
+Section Execution.
+
+  Variable Op: Type -> Type.
+  Variable State : Type.
+
+  Definition OpSemantics := forall T, Op T -> nat -> State -> T -> State -> list event -> Prop.
+  Variable op_step : OpSemantics.
+
+  Definition until1 T (c : T -> bool)
+                      (p : option T -> proc Op T)
+                      (v : option T) :=
+    (* TODO: don't use bool_dec, just do if (c x) ... *)
+    Bind (p v) (fun x => if bool_dec (c x) true then Ret x else Until c p (Some x)).
+
+  Inductive atomic_exec : forall T, proc Op T -> nat -> State ->
+                                    T -> State -> list event -> Prop :=
+
+  | AtomicRet : forall T tid (v : T) s,
+    atomic_exec (Ret v) tid s v s nil
+
+  | AtomicBind : forall T1 T2 tid (p1 : proc Op T1) (p2 : T1 -> proc Op T2)
+                        s0 s1 s2 ev1 ev2 (v1 : T1) (v2 : T2),
+    atomic_exec p1 tid s0 v1 s1 ev1 ->
+    atomic_exec (p2 v1) tid s1 v2 s2 ev2 ->
+    atomic_exec (Bind p1 p2) tid s0 v2 s2 (ev1 ++ ev2)
+
+  | AtomicOp : forall T tid (v : T) s s' op evs,
+    op_step op tid s v s' evs ->
+    atomic_exec (Call op) tid s v s' evs
+
+  | AtomicUntil : forall T (p : option T -> proc Op T) (c : T -> bool) v tid s r s' ev',
+    atomic_exec (until1 c p v) tid s r s' ev' ->
+    atomic_exec (Until c p v) tid s r s' ev'
+  .
+
+  Inductive exec_tid : forall T (tid : nat),
+    State -> proc Op T ->
+    State -> T + proc Op T -> maybe_proc Op -> list event -> Prop :=
+
+  | ExecTidRet : forall tid T (v : T) s,
+    exec_tid tid s (Ret v)
+                 s (inl v)
+                 NoProc nil
+
+  | ExecTidOp : forall tid T (v : T) s s' op evs,
+    op_step op tid s v s' evs ->
+    exec_tid tid s (Call op)
+                 s' (inl v)
+                 NoProc evs
+
+  | ExecTidAtomic : forall tid T (v : T) ap s s' evs,
+    atomic_exec ap tid s v s' evs ->
+    exec_tid tid s (Atomic ap)
+                 s' (inl v)
+                 NoProc evs
+
+  | ExecTidBind : forall tid T1 (p1 : proc Op T1) T2 (p2 : T1 -> proc Op T2) s s' result spawned evs,
+    exec_tid tid s p1
+                 s' result spawned evs ->
+    exec_tid tid s (Bind p1 p2)
+                 s' (inr
+                     match result with
+                     | inl r => p2 r
+                     | inr p1' => Bind p1' p2
+                     end
+                    ) spawned evs
+
+  | ExecTidUntil : forall tid T (p : option T -> proc Op T) (c : T -> bool) v s,
+    exec_tid tid s (Until c p v)
+                 s (inr (until1 c p v))
+                 NoProc nil
+
+  | ExecTidSpawn : forall tid T (p: proc Op T) s,
+    exec_tid tid s (Spawn p)
+                 s (inl tt)
+                 (Proc p) nil
+  .
+
+
+  Inductive exec : State -> threads_state Op -> trace -> Prop :=
+
+  | ExecOne : forall T tid tid' (ts : threads_state Op) trace p s s' evs result spawned,
+    ts tid = @Proc Op T p ->
+    ts tid' = NoProc ->
+    exec_tid tid s p s' result spawned evs ->
+    exec s' (thread_upd (thread_upd ts tid' spawned) tid
+              match result with
+              | inl _ => NoProc
+              | inr p' => Proc p'
+              end) trace ->
+    exec s ts (prepend tid evs trace)
+
+  | ExecStop : forall (ts : threads_state Op) s,
+    exec s ts TraceEmpty.
+
+End Execution.
+
+Hint Constructors exec.
+
+Notation "ts [[ tid ]]" := (thread_get ts tid)
+  (at level 12, left associativity).
+
+Notation "ts [[ tid := p ]]" := (thread_upd ts tid p)
+                                  (at level 12, left associativity).
